Split Sig_noeq.v in half separating the encoding of the congruence in FOL

theories/TRAKHTENBROT/Sig_noeq.v
@@ -16,7 +16,8 @@ From Undecidability.Shared.Libs.DLW.Vec
   Require Import pos vec.
 
 From Undecidability.TRAKHTENBROT
-  Require Import notations utils fol_ops fo_sig fo_terms fo_logic fo_sat.
+  Require Import notations utils fol_ops fo_sig fo_terms 
+                 fo_logic fo_congruence fo_sat.
 
 Set Implicit Arguments.
 
@@ -46,23 +47,7 @@ Set Implicit Arguments.
 
   *)
 
-Section congruence.
-
-  Variables (Σ : fo_signature) (ls : list (syms Σ)) (lr : list (rels Σ))
-            (X : Type) (M : fo_model Σ X)
-            (R : X -> X -> Prop).
-
-  Infix "≈" := R.
-
-  Definition Σ_congruence_wrt :=
-          (forall s, In s ls -> forall v w, (forall p, vec_pos v p ≈ vec_pos w p) 
-                                          -> fom_syms M s v ≈ fom_syms M s w)
-       /\ (forall r, In r lr -> forall v w, (forall p, vec_pos v p ≈ vec_pos w p) 
-                                          -> fom_rels M r v <-> fom_rels M r w).
-
-End congruence.
-
-Section remove_interpreted.
+Section remove_interpreted_symbol.
 
   Variables (Σ : fo_signature) (e : rels Σ) (H_ae : ar_rels _ e = 2)
             (ls : list (syms Σ)) (lr : list (rels Σ))
@@ -73,344 +58,7 @@ Section remove_interpreted.
 
   Notation "x ≡ y" := (@fol_atom Σ e (cast (x##y##ø) (eq_sym H_ae))) (at level 59).
 
-  Section encode_congruence.
-
-    Variable (X : Type) (M : fo_model Σ X).
-
-    Notation "x ≈ y" := (fom_rels M e (cast (x##y##ø) (eq_sym H_ae))).
-
-    Local Fact fol_sem_e x y φ : fol_sem M φ (x ≡ y) = fo_term_sem M φ x ≈ fo_term_sem M φ y.
-    Proof. simpl; f_equal; rewrite H_ae; simpl; auto. Qed.
-
-    Let fol_syms_e x y : fol_syms (x ≡ y) = fo_term_syms x ++ fo_term_syms y.
-    Proof. simpl; rewrite H_ae; simpl; auto; rewrite <- app_nil_end; auto. Qed.
-
-    Let fol_rels_e x y : fol_rels (x ≡ y) = e::nil.
-    Proof. auto. Qed.
-
-    Local Definition fol_vec_equiv n := fol_vec_fa (vec_set_pos (fun p : pos n => £(pos2nat p+n) ≡ £(pos2nat p))).
-
-    Local Fact fol_vec_equiv_syms n : incl (fol_syms (fol_vec_equiv n)) nil.
-    Proof. 
-      unfold fol_vec_equiv.
-      rewrite fol_syms_vec_fa.
-      intros x; rewrite in_flat_map.
-      intros (D & HD & H); revert H.
-      apply vec_list_inv in HD.
-      destruct HD as (p & ->). 
-      rew vec; rewrite fol_syms_e; simpl; tauto.
-    Qed.
-
-    Local Fact fol_vec_equiv_rels n : incl (fol_rels (fol_vec_equiv n)) (e::nil).
-    Proof. 
-      unfold fol_vec_equiv.
-      rewrite fol_rels_vec_fa.
-      intros x; rewrite in_flat_map.
-      intros (D & HD & H); revert H.
-      apply vec_list_inv in HD.
-      destruct HD as (p & ->); rew vec.
-    Qed.
-
-    Local Fact fol_vec_equiv_sem n φ : 
-                fol_sem M φ (fol_vec_equiv n)
-            <-> (forall p : pos n, φ (pos2nat p+n) ≈ φ (pos2nat p)).
-    Proof.
-      unfold fol_vec_equiv.
-      rewrite fol_sem_vec_fa.
-      apply forall_equiv; intros p; rew vec.
-      rewrite fol_sem_e; simpl; tauto.
-    Qed.
-
-    Section congr_syms.
-
-      Variable (s : syms Σ).
-
-      Let n := ar_syms _ s.
-
-      Let A := fol_vec_equiv n.
-      Let f : 𝕋 := in_fot s (vec_set_pos (fun p => £(pos2nat p))).
-      Let g : 𝕋 := in_fot s (vec_set_pos (fun p => £(pos2nat p+n))).
-      Let B := g ≡ f.
-
-      Let HrA : incl (fol_syms A) nil.       Proof. apply fol_vec_equiv_syms. Qed.
-      Let HsA : incl (fol_rels A) (e::nil).  Proof. apply fol_vec_equiv_rels. Qed.
-
-      Let HrB : incl (fol_syms B) (s::nil).
-      Proof.
-        unfold B; simpl.
-        rewrite H_ae; unfold eq_rect_r.
-        intros x; do 2 (simpl; rewrite in_app_iff).
-        do 2 rewrite in_concat_iff.
-        intros [ | [ (l & Hx & H) | [ | [ (l & Hx & H) | [] ] ] ] ]; try tauto; revert Hx;
-          apply vec_list_inv in H; destruct H as (p & ->); rew vec.
-      Qed.
-
-      Let HsB : incl (fol_rels B) (e::nil).
-      Proof. simpl; cbv; tauto. Qed.
-
-      Local Definition congr_syms : 𝔽 := fol_mquant fol_fa n (fol_mquant fol_fa n (A ⤑  B)).
-
-      Local Fact congr_syms_syms : incl (fol_syms congr_syms) (s::nil).
-      Proof.
-        unfold congr_syms.
-        do 2 rewrite fol_syms_mquant.
-        rewrite fol_syms_bin.
-        apply incl_app; auto.
-        intros x Hx; destruct (HrA _ Hx).
-      Qed.
-
-      Local Fact congr_syms_rels : incl (fol_rels congr_syms) (e::nil).
-      Proof.
-        unfold congr_syms.
-        do 2 rewrite fol_rels_mquant.
-        rewrite fol_rels_bin.
-        apply incl_app; auto.
-      Qed.
-
-      Local Definition congr_syms_spec φ : 
-               fol_sem M φ congr_syms
-           <-> forall v w, (forall p, vec_pos v p ≈ vec_pos w p) -> fom_syms M s v ≈ fom_syms M s w.
-      Proof.
-        unfold congr_syms.
-        rewrite fol_sem_mforall.
-        apply forall_equiv; intros v.
-        rewrite fol_sem_mforall.
-        apply forall_equiv; intros w.
-        rewrite fol_sem_bin_fix.
-        apply (fol_bin_sem_ext fol_imp).
-        + unfold A; rewrite fol_vec_equiv_sem.
-          apply forall_equiv; intros p; rew vec; simpl.
-          apply fol_equiv_ext; repeat f_equal.
-          * rewrite env_vlift_fix1, env_vlift_fix0; auto.
-          * rewrite env_vlift_fix0; auto.
-        + unfold B.
-          rewrite fol_sem_e; simpl. 
-          apply fol_equiv_ext; repeat f_equal; 
-            apply vec_pos_ext; intros p; rew vec; rew fot.
-          * rewrite env_vlift_fix1, env_vlift_fix0; auto.
-          * rewrite env_vlift_fix0; auto.
-      Qed.
-
-    End congr_syms.
-
-    Section congr_rels.
-
-      Variable (r : rels Σ).
-
-      Let n := ar_rels _ r.
-
-      Let A := fol_vec_equiv n.
-      Let B := @fol_atom Σ r (vec_set_pos (fun p => £(pos2nat p))).
-      Let C := @fol_atom Σ r (vec_set_pos (fun p => £(pos2nat p+n))).
-
-      Let HsA : incl (fol_syms A) nil.       Proof. apply fol_vec_equiv_syms. Qed.
-      Let HrA : incl (fol_rels A) (e::nil).  Proof. apply fol_vec_equiv_rels. Qed.
-
-      Let HsB : incl (fol_syms B) nil.
-      Proof.
-        unfold B; simpl.
-        intros x; rewrite in_flat_map.
-        intros (t & H & Ht); revert Ht.
-        apply vec_list_inv in H; destruct H as (p & ->); rew vec.
-      Qed.
-
-      Let HrB : incl (fol_rels B) (r::nil).
-      Proof. simpl; cbv; tauto. Qed.
-
-      Let HsC : incl (fol_syms C) nil.
-      Proof. 
-        unfold C; simpl.
-        intros x; rewrite in_flat_map.
-        intros (t & Ht & H); revert H.
-        apply vec_list_inv in Ht.
-        destruct Ht as (p & ->); rew vec; simpl; tauto.
-      Qed.
-
-      Let HrC : incl (fol_rels C) (e::r::nil).
-      Proof. simpl; cbv; tauto. Qed.
-
-      Local Definition congr_rels : 𝔽 := fol_mquant fol_fa n (fol_mquant fol_fa n (A ⤑  (C ↔ B))).
-
-      Local Fact congr_rels_syms : incl (fol_syms congr_rels) nil.
-      Proof.
-        unfold congr_rels.
-        do 2 rewrite fol_syms_mquant.
-        repeat rewrite fol_syms_bin.
-        repeat (apply incl_app; auto).
-      Qed.
-
-      Local Fact congr_rels_rels : incl (fol_rels congr_rels) (e::r::nil).
-      Proof.
-        unfold congr_rels.
-        do 2 rewrite fol_rels_mquant.
-        repeat rewrite fol_rels_bin.
-        repeat (apply incl_app; auto).
-        intros x Hx; destruct (HrA _ Hx); try subst x; simpl; tauto.
-      Qed.
-
-      Local Definition congr_rels_spec φ : 
-             fol_sem M φ congr_rels
-         <-> forall v w, (forall p, vec_pos v p ≈ vec_pos w p) 
-                      -> fom_rels M r v <-> fom_rels M r w.
-      Proof.
-        unfold congr_rels.
-        rewrite fol_sem_mforall.
-        apply forall_equiv; intros v.
-        rewrite fol_sem_mforall.
-        apply forall_equiv; intros w.
-        simpl fol_sem at 1.
-        apply (fol_bin_sem_ext fol_imp).
-        + unfold A; rewrite fol_vec_equiv_sem.
-          apply forall_equiv; intros p; rew vec; simpl.
-          apply fol_equiv_ext; repeat f_equal.
-          * rewrite env_vlift_fix1, env_vlift_fix0; auto.
-          * rewrite env_vlift_fix0; auto.
-        + apply fol_equiv_sem_ext; apply fol_equiv_ext; f_equal;
-            apply vec_pos_ext; intros p; rew vec; rew fot.
-          * rewrite env_vlift_fix1, env_vlift_fix0; auto.
-          * rewrite env_vlift_fix0; auto.
-      Qed.
-
-    End congr_rels.
-
-    Definition Σ_eq_congruent : 𝔽 :=
-        fol_lconj (map congr_syms ls) 
-      ⟑ fol_lconj (map congr_rels lr).
-
-    Fact Σ_eq_congruent_syms : incl (fol_syms Σ_eq_congruent) ls.
-    Proof.
-      unfold Σ_eq_congruent.
-      rewrite fol_syms_bin.
-      repeat rewrite fol_syms_bigop; simpl.
-      repeat apply incl_app; try (cbv; tauto).
-      + intros s; rewrite in_flat_map.
-        intros (A & HA & H); revert HA H.
-        rewrite in_map_iff; intros (x & <- & Hx) H.
-        apply congr_syms_syms in H; revert H.
-        intros [ <- | [] ]; auto.
-      + intros r; rewrite in_flat_map.
-        intros (A & HA & H); revert HA H.
-        rewrite in_map_iff; intros (x & <- & Hx) H.
-        apply congr_rels_syms in H; revert H.
-        intros [].
-    Qed.
-
-    Fact Σ_eq_congruent_rels : incl (fol_rels Σ_eq_congruent) lr.
-    Proof.
-      unfold Σ_eq_congruent.
-      rewrite fol_rels_bin.
-      repeat rewrite fol_rels_bigop; simpl.
-      repeat apply incl_app; try (cbv; tauto).
-      + intros s; rewrite in_flat_map.
-        intros (A & HA & H); revert HA H.
-        rewrite in_map_iff; intros (x & <- & Hx) H.
-        apply congr_syms_rels in H; revert H.
-        intros [ <- | [] ]; simpl; auto.
-      + intros x; simpl.
-        rewrite in_flat_map.
-        intros (A & HA & H); revert HA H.
-        rewrite in_map_iff; intros (y & <- & Hy) H.
-        apply congr_rels_rels in H; revert H.
-        intros [ | [ <- | [] ] ]; subst; auto.
-    Qed.
-
-    (** Σ_eq_congruence_spec encodes that ≈ is a congruence wrt to all
-        the symbols in ls and lr *)
-
-    Fact Σ_eq_congruent_spec φ :
-          fol_sem M φ Σ_eq_congruent 
-      <-> Σ_congruence_wrt ls lr M (fun x y => x ≈ y).
-    Proof.
-      unfold Σ_eq_congruent.
-      rewrite fol_sem_bin_fix.
-      do 2 rewrite fol_sem_lconj.
-      apply (fol_bin_sem_ext fol_conj).
-      + split.
-        * intros H s Hs.
-          apply (congr_syms_spec _ φ), H, in_map_iff.
-          exists s; auto.
-        * intros H f; rewrite in_map_iff.
-          intros (s & <- & Hs).
-          apply congr_syms_spec, H; auto.
-      + split.
-        * intros H r Hr.
-          apply (congr_rels_spec _ φ), H, in_map_iff.
-          exists r; auto.
-        * intros H f; rewrite in_map_iff.
-          intros (r & <- & Hr).
-          apply congr_rels_spec, H; auto.
-    Qed.
-
-    Definition Σ_eq_equivalence := 
-            (∀ £0 ≡ £0)
-          ⟑ (∀∀∀ £2 ≡ £1 ⤑ £1 ≡ £0 ⤑ £2 ≡ £0)
-          ⟑ (∀∀ £1 ≡ £0 ⤑ £0 ≡ £1).
-
-    Local Fact Σ_eq_equivalence_syms : fol_syms Σ_eq_equivalence = nil.
-    Proof.
-      unfold Σ_eq_equivalence.
-      repeat (rewrite fol_syms_bin || rewrite fol_syms_quant).
-      repeat rewrite fol_syms_e; auto.
-    Qed.
-
-    Local Fact Σ_eq_equivalence_rels : incl (fol_rels Σ_eq_equivalence) (e::nil).
-    Proof. simpl; cbv; tauto. Qed.
-  
-    Fact Σ_eq_equiv_spec φ : 
-           fol_sem M φ Σ_eq_equivalence <-> equiv _ (fun x y => x ≈ y).
-    Proof.
-      unfold Σ_eq_equivalence.
-      repeat (rewrite fol_sem_bin_fix).
-      repeat apply fol_bin_sem_ext.
-      + rewrite fol_sem_quant_fix; apply forall_equiv; intro.
-        rewrite fol_sem_e; simpl; tauto.
-      + do 3 (rewrite fol_sem_quant_fix; apply forall_equiv; intro).
-        do 2 rewrite fol_sem_bin_fix.
-        do 3 rewrite fol_sem_e; simpl; tauto.
-      + do 2 (rewrite fol_sem_quant_fix; apply forall_equiv; intro).
-        rewrite fol_sem_bin_fix.
-        do 2 rewrite fol_sem_e; simpl; tauto.
-    Qed.
-
-    (** Σ_eq_congruence encodes the fact that ≈ is a congruence wrt to all
-        the symbols in ls and lr and this formula involve only the symbols
-        of ls and lr, under the assumption that e belongs to lr *)
-
-    Definition Σ_eq_congruence := 
-          Σ_eq_congruent 
-        ⟑ Σ_eq_equivalence.
-
-    Fact Σ_eq_congruence_syms : incl (fol_syms Σ_eq_congruence) ls.
-    Proof.
-      unfold Σ_eq_congruence.
-      rewrite fol_syms_bin, Σ_eq_equivalence_syms, <- app_nil_end.
-      apply Σ_eq_congruent_syms.
-    Qed.
-
-    Fact Σ_eq_congruence_rels : incl (fol_rels Σ_eq_congruence) lr.
-    Proof.
-      unfold Σ_eq_congruence.
-      rewrite fol_rels_bin.
-      apply incl_app.
-      + apply Σ_eq_congruent_rels.
-      + intros x Hx.
-        apply Σ_eq_equivalence_rels in Hx.
-        destruct Hx as [ | [] ]; subst; auto.
-    Qed.
-
-    Fact Σ_eq_congruence_spec φ : 
-             fol_sem M φ Σ_eq_congruence
-         <-> Σ_congruence_wrt ls lr M (fun x y => x ≈ y)
-          /\ equiv _ (fun x y => x ≈ y).
-    Proof.
-      apply fol_bin_sem_ext.
-      + apply Σ_eq_congruent_spec.
-      + apply Σ_eq_equiv_spec.
-    Qed.
-
-  End encode_congruence.
-
-  Definition Σ_noeq A := Σ_eq_congruence ⟑ A.
+  Definition Σ_noeq A := fol_congruence H_ae ls lr ⟑ A.
 
   Section soundness.
 
@@ -423,8 +71,9 @@ Section remove_interpreted.
       intros (M & H1 & H2 & HE & phi & H5).
       exists M, H1, H2, phi; unfold Σ_noeq.
       rewrite fol_sem_bin_fix; split; auto.
+      rewrite fol_sem_congruence.
       split; [ | msplit 2 ].
-      + rewrite Σ_eq_congruent_spec; split.
+      + split.
         * intros s _ v w H; rewrite HE.
           f_equal; apply vec_pos_ext; intros p.
           apply HE, H.
@@ -432,13 +81,9 @@ Section remove_interpreted.
           apply fol_equiv_ext; f_equal.
           apply vec_pos_ext; intros p.
           apply HE, H.
-      + intros ?; rewrite fol_sem_e, HE; auto.
-      + intros ? ? ?; repeat rewrite fol_sem_bin_fix.
-        do 3 rewrite fol_sem_e; simpl.
-        repeat rewrite HE; intros; subst; auto.
-      + intros ? ?; rewrite fol_sem_bin_fix.
-        do 2 rewrite fol_sem_e; simpl.
-        now repeat rewrite HE.
+      + intros ?; rewrite HE; auto.
+      + intros ? ? ?; rewrite !HE; intros; subst; auto.
+      + intros ? ?; rewrite !HE; intros; subst; auto.
     Qed.
 
   End soundness.
@@ -458,11 +103,9 @@ Section remove_interpreted.
                fo_form_fin_dec_SAT (Σ_noeq A)
             -> fo_form_fin_dec_eq_SAT e H_ae A.
     Proof.
-      intros (X & M & H1 & H2 & phi & (H5 & H6) & H3).
-      apply Σ_eq_congruent_spec in H5.
-      destruct H5 as (H4 & H5).
-      apply Σ_eq_equiv_spec in H6.
-      destruct H6 as (H6 & H8 & H7).
+      intros (X & M & H1 & H2 & phi & H5 & H3).
+      apply fol_sem_congruence in H5.
+      destruct H5 as ((H4 & H5) & (H6 & H8 & H7)).
       set (R x y := fom_rels M e (cast (x ## y ## ø) (eq_sym H_ae))).
       destruct H1 as (lX & HlX).
       destruct decidable_EQUIV_fin_quotient with (l := lX) (R := R)
@@ -498,5 +141,5 @@ Section remove_interpreted.
 
   End completeness.
 
-End remove_interpreted.
+End remove_interpreted_symbol.
 
