theories/TRAKHTENBROT/fo_congruence.v
@@ -1,0 +1,392 @@
+(**************************************************************)
+(*   Copyright Dominique Larchey-Wendling [*]                 *)
+(*                                                            *)
+(*                             [*] Affiliation LORIA -- CNRS  *)
+(**************************************************************)
+(*      This file is distributed under the terms of the       *)
+(*         CeCILL v2 FREE SOFTWARE LICENSE AGREEMENT          *)
+(**************************************************************)
+
+Require Import List Arith Lia Relations.
+
+From Undecidability.Shared.Libs.DLW.Utils
+  Require Import utils_tac utils_list utils_nat finite.
+
+From Undecidability.Shared.Libs.DLW.Vec 
+  Require Import pos vec.
+
+From Undecidability.TRAKHTENBROT
+  Require Import notations utils fol_ops fo_sig fo_terms fo_logic.
+
+Set Implicit Arguments.
+
+Section congruence.
+
+  Variables (Σ : fo_signature) (ls : list (syms Σ)) (lr : list (rels Σ))
+            (X : Type) (M : fo_model Σ X)
+            (R : X -> X -> Prop).
+
+  Infix "≈" := R.
+
+  Definition Σ_congruence_wrt :=
+          (forall s, In s ls -> forall v w, (forall p, vec_pos v p ≈ vec_pos w p) 
+                                          -> fom_syms M s v ≈ fom_syms M s w)
+       /\ (forall r, In r lr -> forall v w, (forall p, vec_pos v p ≈ vec_pos w p) 
+                                          -> fom_rels M r v <-> fom_rels M r w).
+
+End congruence.
+
+Section fol_congruence.
+
+  Variables (Σ : fo_signature) (e : rels Σ) (H_ae : ar_rels _ e = 2)
+            (ls : list (syms Σ)) (lr : list (rels Σ))
+            (He : In e lr). 
+
+  Notation 𝕋 := (fol_term Σ).
+  Notation 𝔽 := (fol_form Σ).
+
+  Notation "x ≡ y" := (@fol_atom Σ e (cast (x##y##ø) (eq_sym H_ae))) (at level 59).
+
+  Section encode_congruence.
+
+    Variable (X : Type) (M : fo_model Σ X).
+
+    Notation "x ≈ y" := (fom_rels M e (cast (x##y##ø) (eq_sym H_ae))).
+
+    Local Fact fol_sem_e x y φ : fol_sem M φ (x ≡ y) = fo_term_sem M φ x ≈ fo_term_sem M φ y.
+    Proof. simpl; f_equal; rewrite H_ae; simpl; auto. Qed.
+
+    Let fol_syms_e x y : fol_syms (x ≡ y) = fo_term_syms x ++ fo_term_syms y.
+    Proof. simpl; rewrite H_ae; simpl; auto; rewrite <- app_nil_end; auto. Qed.
+
+    Let fol_rels_e x y : fol_rels (x ≡ y) = e::nil.
+    Proof. auto. Qed.
+
+    Local Definition fol_vec_equiv n := fol_vec_fa (vec_set_pos (fun p : pos n => £(pos2nat p+n) ≡ £(pos2nat p))).
+
+    Local Fact fol_vec_equiv_syms n : incl (fol_syms (fol_vec_equiv n)) nil.
+    Proof. 
+      unfold fol_vec_equiv.
+      rewrite fol_syms_vec_fa.
+      intros x; rewrite in_flat_map.
+      intros (D & HD & H); revert H.
+      apply vec_list_inv in HD.
+      destruct HD as (p & ->). 
+      rew vec; rewrite fol_syms_e; simpl; tauto.
+    Qed.
+
+    Local Fact fol_vec_equiv_rels n : incl (fol_rels (fol_vec_equiv n)) (e::nil).
+    Proof. 
+      unfold fol_vec_equiv.
+      rewrite fol_rels_vec_fa.
+      intros x; rewrite in_flat_map.
+      intros (D & HD & H); revert H.
+      apply vec_list_inv in HD.
+      destruct HD as (p & ->); rew vec.
+    Qed.
+
+    Local Fact fol_vec_equiv_sem n φ : 
+                fol_sem M φ (fol_vec_equiv n)
+            <-> (forall p : pos n, φ (pos2nat p+n) ≈ φ (pos2nat p)).
+    Proof.
+      unfold fol_vec_equiv.
+      rewrite fol_sem_vec_fa.
+      apply forall_equiv; intros p; rew vec.
+      rewrite fol_sem_e; simpl; tauto.
+    Qed.
+
+    Section congr_syms.
+
+      Variable (s : syms Σ).
+
+      Let n := ar_syms _ s.
+
+      Let A := fol_vec_equiv n.
+      Let f : 𝕋 := in_fot s (vec_set_pos (fun p => £(pos2nat p))).
+      Let g : 𝕋 := in_fot s (vec_set_pos (fun p => £(pos2nat p+n))).
+      Let B := g ≡ f.
+
+      Let HrA : incl (fol_syms A) nil.       Proof. apply fol_vec_equiv_syms. Qed.
+      Let HsA : incl (fol_rels A) (e::nil).  Proof. apply fol_vec_equiv_rels. Qed.
+
+      Let HrB : incl (fol_syms B) (s::nil).
+      Proof.
+        unfold B; simpl.
+        rewrite H_ae; unfold eq_rect_r.
+        intros x; do 2 (simpl; rewrite in_app_iff).
+        do 2 rewrite in_concat_iff.
+        intros [ | [ (l & Hx & H) | [ | [ (l & Hx & H) | [] ] ] ] ]; try tauto; revert Hx;
+          apply vec_list_inv in H; destruct H as (p & ->); rew vec.
+      Qed.
+
+      Let HsB : incl (fol_rels B) (e::nil).
+      Proof. simpl; cbv; tauto. Qed.
+
+      Local Definition congr_syms : 𝔽 := fol_mquant fol_fa n (fol_mquant fol_fa n (A ⤑  B)).
+
+      Local Fact congr_syms_syms : incl (fol_syms congr_syms) (s::nil).
+      Proof.
+        unfold congr_syms.
+        do 2 rewrite fol_syms_mquant.
+        rewrite fol_syms_bin.
+        apply incl_app; auto.
+        intros x Hx; destruct (HrA _ Hx).
+      Qed.
+
+      Local Fact congr_syms_rels : incl (fol_rels congr_syms) (e::nil).
+      Proof.
+        unfold congr_syms.
+        do 2 rewrite fol_rels_mquant.
+        rewrite fol_rels_bin.
+        apply incl_app; auto.
+      Qed.
+
+      Local Definition congr_syms_spec φ : 
+               fol_sem M φ congr_syms
+           <-> forall v w, (forall p, vec_pos v p ≈ vec_pos w p) -> fom_syms M s v ≈ fom_syms M s w.
+      Proof.
+        unfold congr_syms.
+        rewrite fol_sem_mforall.
+        apply forall_equiv; intros v.
+        rewrite fol_sem_mforall.
+        apply forall_equiv; intros w.
+        rewrite fol_sem_bin_fix.
+        apply (fol_bin_sem_ext fol_imp).
+        + unfold A; rewrite fol_vec_equiv_sem.
+          apply forall_equiv; intros p; rew vec; simpl.
+          apply fol_equiv_ext; repeat f_equal.
+          * rewrite env_vlift_fix1, env_vlift_fix0; auto.
+          * rewrite env_vlift_fix0; auto.
+        + unfold B.
+          rewrite fol_sem_e; simpl. 
+          apply fol_equiv_ext; repeat f_equal; 
+            apply vec_pos_ext; intros p; rew vec; rew fot.
+          * rewrite env_vlift_fix1, env_vlift_fix0; auto.
+          * rewrite env_vlift_fix0; auto.
+      Qed.
+
+    End congr_syms.
+
+    Section congr_rels.
+
+      Variable (r : rels Σ).
+
+      Let n := ar_rels _ r.
+
+      Let A := fol_vec_equiv n.
+      Let B := @fol_atom Σ r (vec_set_pos (fun p => £(pos2nat p))).
+      Let C := @fol_atom Σ r (vec_set_pos (fun p => £(pos2nat p+n))).
+
+      Let HsA : incl (fol_syms A) nil.       Proof. apply fol_vec_equiv_syms. Qed.
+      Let HrA : incl (fol_rels A) (e::nil).  Proof. apply fol_vec_equiv_rels. Qed.
+
+      Let HsB : incl (fol_syms B) nil.
+      Proof.
+        unfold B; simpl.
+        intros x; rewrite in_flat_map.
+        intros (t & H & Ht); revert Ht.
+        apply vec_list_inv in H; destruct H as (p & ->); rew vec.
+      Qed.
+
+      Let HrB : incl (fol_rels B) (r::nil).
+      Proof. simpl; cbv; tauto. Qed.
+
+      Let HsC : incl (fol_syms C) nil.
+      Proof. 
+        unfold C; simpl.
+        intros x; rewrite in_flat_map.
+        intros (t & Ht & H); revert H.
+        apply vec_list_inv in Ht.
+        destruct Ht as (p & ->); rew vec; simpl; tauto.
+      Qed.
+
+      Let HrC : incl (fol_rels C) (e::r::nil).
+      Proof. simpl; cbv; tauto. Qed.
+
+      Local Definition congr_rels : 𝔽 := fol_mquant fol_fa n (fol_mquant fol_fa n (A ⤑  (C ↔ B))).
+
+      Local Fact congr_rels_syms : incl (fol_syms congr_rels) nil.
+      Proof.
+        unfold congr_rels.
+        do 2 rewrite fol_syms_mquant.
+        repeat rewrite fol_syms_bin.
+        repeat (apply incl_app; auto).
+      Qed.
+
+      Local Fact congr_rels_rels : incl (fol_rels congr_rels) (e::r::nil).
+      Proof.
+        unfold congr_rels.
+        do 2 rewrite fol_rels_mquant.
+        repeat rewrite fol_rels_bin.
+        repeat (apply incl_app; auto).
+        intros x Hx; destruct (HrA _ Hx); try subst x; simpl; tauto.
+      Qed.
+
+      Local Definition congr_rels_spec φ : 
+             fol_sem M φ congr_rels
+         <-> forall v w, (forall p, vec_pos v p ≈ vec_pos w p) 
+                      -> fom_rels M r v <-> fom_rels M r w.
+      Proof.
+        unfold congr_rels.
+        rewrite fol_sem_mforall.
+        apply forall_equiv; intros v.
+        rewrite fol_sem_mforall.
+        apply forall_equiv; intros w.
+        simpl fol_sem at 1.
+        apply (fol_bin_sem_ext fol_imp).
+        + unfold A; rewrite fol_vec_equiv_sem.
+          apply forall_equiv; intros p; rew vec; simpl.
+          apply fol_equiv_ext; repeat f_equal.
+          * rewrite env_vlift_fix1, env_vlift_fix0; auto.
+          * rewrite env_vlift_fix0; auto.
+        + apply fol_equiv_sem_ext; apply fol_equiv_ext; f_equal;
+            apply vec_pos_ext; intros p; rew vec; rew fot.
+          * rewrite env_vlift_fix1, env_vlift_fix0; auto.
+          * rewrite env_vlift_fix0; auto.
+      Qed.
+
+    End congr_rels.
+
+    Local Definition fol_congruent : 𝔽 :=
+        fol_lconj (map congr_syms ls) 
+      ⟑ fol_lconj (map congr_rels lr).
+
+    Local Fact fol_congruent_syms : incl (fol_syms fol_congruent) ls.
+    Proof.
+      unfold fol_congruent.
+      rewrite fol_syms_bin.
+      repeat rewrite fol_syms_bigop; simpl.
+      repeat apply incl_app; try (cbv; tauto).
+      + intros s; rewrite in_flat_map.
+        intros (A & HA & H); revert HA H.
+        rewrite in_map_iff; intros (x & <- & Hx) H.
+        apply congr_syms_syms in H; revert H.
+        intros [ <- | [] ]; auto.
+      + intros r; rewrite in_flat_map.
+        intros (A & HA & H); revert HA H.
+        rewrite in_map_iff; intros (x & <- & Hx) H.
+        apply congr_rels_syms in H; revert H.
+        intros [].
+    Qed.
+
+    Local Fact fol_congruent_rels : incl (fol_rels fol_congruent) lr.
+    Proof.
+      unfold fol_congruent.
+      rewrite fol_rels_bin.
+      repeat rewrite fol_rels_bigop; simpl.
+      repeat apply incl_app; try (cbv; tauto).
+      + intros s; rewrite in_flat_map.
+        intros (A & HA & H); revert HA H.
+        rewrite in_map_iff; intros (x & <- & Hx) H.
+        apply congr_syms_rels in H; revert H.
+        intros [ <- | [] ]; simpl; auto.
+      + intros x; simpl.
+        rewrite in_flat_map.
+        intros (A & HA & H); revert HA H.
+        rewrite in_map_iff; intros (y & <- & Hy) H.
+        apply congr_rels_rels in H; revert H.
+        intros [ | [ <- | [] ] ]; subst; auto.
+    Qed.
+
+    (** Σ_eq_congruence_spec encodes that ≈ is a congruence wrt to all
+        the symbols in ls and lr *)
+
+    Local Fact fol_congruent_spec φ :
+          fol_sem M φ fol_congruent 
+      <-> Σ_congruence_wrt ls lr M (fun x y => x ≈ y).
+    Proof.
+      unfold fol_congruent.
+      rewrite fol_sem_bin_fix.
+      do 2 rewrite fol_sem_lconj.
+      apply (fol_bin_sem_ext fol_conj).
+      + split.
+        * intros H s Hs.
+          apply (congr_syms_spec _ φ), H, in_map_iff.
+          exists s; auto.
+        * intros H f; rewrite in_map_iff.
+          intros (s & <- & Hs).
+          apply congr_syms_spec, H; auto.
+      + split.
+        * intros H r Hr.
+          apply (congr_rels_spec _ φ), H, in_map_iff.
+          exists r; auto.
+        * intros H f; rewrite in_map_iff.
+          intros (r & <- & Hr).
+          apply congr_rels_spec, H; auto.
+    Qed.
+
+    Local Definition fol_equivalence := 
+            (∀ £0 ≡ £0)
+          ⟑ (∀∀∀ £2 ≡ £1 ⤑ £1 ≡ £0 ⤑ £2 ≡ £0)
+          ⟑ (∀∀ £1 ≡ £0 ⤑ £0 ≡ £1).
+
+    Local Fact fol_equivalence_syms : fol_syms fol_equivalence = nil.
+    Proof.
+      unfold fol_equivalence.
+      repeat (rewrite fol_syms_bin || rewrite fol_syms_quant).
+      repeat rewrite fol_syms_e; auto.
+    Qed.
+
+    Local Fact fol_equivalence_rels : incl (fol_rels fol_equivalence) (e::nil).
+    Proof. simpl; cbv; tauto. Qed.
+  
+    Fact fol_equiv_spec φ : 
+           fol_sem M φ fol_equivalence <-> equiv _ (fun x y => x ≈ y).
+    Proof.
+      unfold fol_equivalence.
+      repeat (rewrite fol_sem_bin_fix).
+      repeat apply fol_bin_sem_ext.
+      + rewrite fol_sem_quant_fix; apply forall_equiv; intro.
+        rewrite fol_sem_e; simpl; tauto.
+      + do 3 (rewrite fol_sem_quant_fix; apply forall_equiv; intro).
+        do 2 rewrite fol_sem_bin_fix.
+        do 3 rewrite fol_sem_e; simpl; tauto.
+      + do 2 (rewrite fol_sem_quant_fix; apply forall_equiv; intro).
+        rewrite fol_sem_bin_fix.
+        do 2 rewrite fol_sem_e; simpl; tauto.
+    Qed.
+
+    (** Σ_eq_congruence encodes the fact that ≈ is a congruence wrt to all
+        the symbols in ls and lr and this formula involve only the symbols
+        of ls and lr, under the assumption that e belongs to lr *)
+
+    Definition fol_congruence := 
+          fol_congruent 
+        ⟑ fol_equivalence.
+
+    Fact fol_congruence_syms : incl (fol_syms fol_congruence) ls.
+    Proof.
+      unfold fol_congruence.
+      rewrite fol_syms_bin, fol_equivalence_syms, <- app_nil_end.
+      apply fol_congruent_syms.
+    Qed.
+
+    Fact fol_congruence_rels : incl (fol_rels fol_congruence) lr.
+    Proof.
+      unfold fol_congruence.
+      rewrite fol_rels_bin.
+      apply incl_app.
+      + apply fol_congruent_rels.
+      + intros x Hx.
+        apply fol_equivalence_rels in Hx.
+        destruct Hx as [ | [] ]; subst; auto.
+    Qed.
+
+    Fact fol_sem_congruence φ : 
+             fol_sem M φ fol_congruence
+         <-> Σ_congruence_wrt ls lr M (fun x y => x ≈ y)
+          /\ equiv _ (fun x y => x ≈ y).
+    Proof.
+      apply fol_bin_sem_ext.
+      + apply fol_congruent_spec.
+      + apply fol_equiv_spec.
+    Qed.
+
+  End encode_congruence.
+
+End fol_congruence.
+
+Arguments fol_congruence { _ _ }.
+
+Print fol_congruence.
+
